WIP in inline proof

theories/L6_PCPS/inline_correct.v
@@ -118,13 +118,43 @@ End Inline_Eq.
 
 Opaque bind ret.
 
- 
+
+Definition Range (x1 x2 : positive) : Ensemble var := fun z => x1 <= z < x2.
+
+Lemma Disjoint_Range (x1 x2 x1' x2' : positive) :
+  x2 <= x1' ->
+  Disjoint _ (Range x1 x2) (Range x1' x2').
+Proof.
+  intros Hleq. constructor. intros x Hin. inv Hin.
+  unfold Range, Ensembles.In in *. simpl in *. zify. omega.
+Qed.    
+
+Lemma Range_Subset (x1 x2 x1' x2' : positive) :
+  x1 <= x1' ->
+  x2' <= x2 ->
+  Range x1' x2' \subset Range x1 x2.
+Proof.
+  intros H1 H2. intros z Hin. unfold Range, Ensembles.In in *.
+  inv Hin. zify. omega.
+Qed.
+        
+  
+Lemma fresh_Range S (x1 x2 : positive) :
+  fresh S x1 ->
+  Range x1 x2 \subset S.
+Proof.
+  intros Hin z Hin'. inv Hin'. eapply Hin. eassumption.
+Qed.
+
 (** Spec for [get_name] *)
 Lemma get_name_fresh A S y str :
   {{ fun _ (s : comp_data * A) => fresh S (next_var (fst s)) }}
     get_name y str
-  {{ fun (r: unit) _ x s' =>
-       x \in S /\ fresh (S \\ [set x]) (next_var (fst s')) }}.  
+  {{ fun (r: unit) s x s' =>
+       x \in Range (next_var (fst s)) (next_var (fst s')) /\
+       (next_var (fst s) < next_var (fst s')) /\
+       fresh (S \\ [set x]) (next_var (fst s'))      
+  }}.  
 Proof. 
   eapply pre_post_mp_l.
   eapply bind_triple. now eapply get_triple.  
@@ -134,28 +164,37 @@ Proof.
   intros x [r3 w3].
   eapply return_triple. 
   intros ? [r4 w4] H2. inv H2. intros [H1 H2]. inv H1; inv H2. intros.
-  split. eapply H. reflexivity. 
-  simpl. intros z Hin. constructor. eapply H; eauto. zify. omega.
+  split. simpl. unfold Range, Ensembles.In. zify. omega.
+  simpl. split. zify; omega.
+  intros z Hin. constructor. eapply H; eauto. zify. omega.
   intros Hc. inv Hc. zify; omega.
 Qed.
 
 Lemma get_names_lst_fresh A S ns str :
   {{ fun _ (s : comp_data * A) => fresh S (next_var (fst s)) }}
-     get_names_lst ns str
-  {{ fun (r: unit) _ xs s' =>
-       FromList xs \subset S /\ NoDup xs /\ fresh (S \\ FromList xs) (next_var (fst s')) }}.  
+    get_names_lst ns str
+  {{ fun (r: unit) s xs s' =>
+       NoDup xs /\ List.length xs = List.length ns /\
+       FromList xs \subset Range (next_var (fst s)) (next_var (fst s')) /\
+       (next_var (fst s) <= next_var (fst s')) /\
+       fresh (S \\ FromList xs) (next_var (fst s')) }}.  
 Proof.
   unfold get_names_lst. revert S; induction ns; intros S.
   - simpl. eapply return_triple.
-    intros. repeat normalize_sets. split; eauto. sets. split; eauto.
-    now constructor.
+    intros. repeat normalize_sets. split; eauto. sets. now constructor. split; eauto.
+    split. now sets. split. reflexivity. eassumption.
   - simpl. eapply bind_triple. eapply get_name_fresh.
-    intros x w. eapply pre_curry_l. intros Hin.
-    eapply bind_triple. eapply IHns.
+    intros x w.
+    eapply bind_triple. eapply frame_rule. eapply frame_rule. eapply IHns.
     intros xs w'. eapply return_triple. intros. destructAll.
-    repeat normalize_sets. split; [| split ].
-    + eapply Union_Included. now sets. eapply Included_trans. eassumption. sets.
-    + constructor; eauto. intros hc. eapply H. eassumption. sets.
+    repeat normalize_sets. split; [| split; [| split; [| split ]]].
+    + constructor; eauto. intros Hc. eapply H3 in Hc. 
+      eapply Disjoint_Range; [| constructor; [ eapply H | eapply Hc ] ]. reflexivity.
+    + simpl. omega.
+    + eapply Union_Included. eapply Singleton_Included.
+      eapply Range_Subset; [| | eassumption ]. reflexivity. zify. omega.
+      eapply Included_trans. eassumption. eapply Range_Subset. zify; omega. reflexivity.
+    + zify; omega.
     + rewrite <- Setminus_Union. eassumption.
 Qed.
   
@@ -207,9 +246,6 @@ Section Inline_correct.
     | Vfun rho B f => occurs_free_fundefs B :|: name_in_fundefs B
     | _ => Empty_set _
     end.
-    
-  Definition occurs_free_in_env (rho : env) : Ensemble var :=
-    fun v => exists x r B f, rho!x = Some (Vfun r B f) /\ v \in occurs_free_fundefs B :|: name_in_fundefs B.
 
   Definition fun_bindings_val (v : val) :=
     match v with
@@ -272,19 +308,26 @@ Section Inline_correct.
     - simpl in HIn. now right.
   Qed.
 
+  Definition occurs_free_fun_map (fm : fun_map) : Ensemble var :=
+    fun x => exists f ft xs e, fm ! f = Some (ft, xs, e) /\ x \in occurs_free e \\ FromList xs.
+
+  Definition bound_var_fun_map (fm : fun_map) : Ensemble var :=
+    fun x => exists f ft xs e, fm ! f = Some (ft, xs, e) /\ x \in bound_var e :|: FromList xs.
+
+
   Fixpoint fun_map_inv' (k : nat) (S : Ensemble var) (fm : fun_map) (rho1 rho2 : env) (i : nat) (sig : subst) : Prop :=
     forall f ft xs e rhoc B f',
       f \in S ->
       fm ! f = Some (ft, xs, e) ->
       rho1 ! f = Some (Vfun rhoc B f') ->
       find_def f B = Some (ft, xs, e) /\ f = f' /\
-      preord_env_P_inj cenv PG (name_in_fundefs B :|: occurs_free_fundefs B) i (apply_r sig) (def_funs B B rhoc rhoc) rho2 /\
+      preord_env_P_inj cenv PG (occurs_free e \\ FromList xs) i (apply_r sig) (def_funs B B rhoc rhoc) rho2 /\
       sub_map (def_funs B B rhoc rhoc) rho1 /\
-      Disjoint _ (bound_var e) (name_in_fundefs B :|: FromList xs :|: occurs_free_in_env rho1 :|: Dom_map rhoc) /\
-      Disjoint _ (FromList xs) (name_in_fundefs B :|: occurs_free_in_env rho1 :|: Dom_map rhoc :|: Dom_map fm) /\
+      Disjoint _ (bound_var e) (FromList xs :|: Dom_map rhoc :|: name_in_fundefs B) /\
+      Disjoint _ (FromList xs) (Dom_map rhoc :|: Dom_map fm :|: name_in_fundefs B) /\
       match k with
       | 0%nat => True
-      | S k => fun_map_inv' k (occurs_free_in_env rho1) fm (def_funs B B rhoc rhoc) rho2 i sig
+      | S k => fun_map_inv' k (occurs_free e \\ FromList xs) fm (def_funs B B rhoc rhoc) rho2 i sig
       end.
 
   Definition fun_map_inv (k : nat) (S : Ensemble var) (fm : fun_map) (rho1 rho2 : env) (i : nat) (sig : subst) : Prop :=
@@ -293,13 +336,13 @@ Section Inline_correct.
       fm ! f = Some (ft, xs, e) ->
       rho1 ! f = Some (Vfun rhoc B f') ->
       find_def f B = Some (ft, xs, e) /\ f = f' /\
-      preord_env_P_inj cenv PG (name_in_fundefs B :|: occurs_free_fundefs B) i (apply_r sig) (def_funs B B rhoc rhoc) rho2 /\
+      preord_env_P_inj cenv PG (occurs_free e \\ FromList xs) i (apply_r sig) (def_funs B B rhoc rhoc) rho2 /\
       sub_map (def_funs B B rhoc rhoc) rho1 /\
-      Disjoint _ (bound_var e) (name_in_fundefs B :|: FromList xs :|: occurs_free_in_env rho1 :|: Dom_map rhoc) /\
-      Disjoint _ (FromList xs) (name_in_fundefs B :|: occurs_free_in_env rho1 :|: Dom_map rhoc :|: Dom_map fm) /\
+      Disjoint _ (bound_var e) (FromList xs :|: Dom_map rhoc :|: name_in_fundefs B) /\
+      Disjoint _ (FromList xs) (Dom_map rhoc :|: Dom_map fm :|: name_in_fundefs B) /\
       match k with
       | 0%nat => True
-      | S k => fun_map_inv' k (occurs_free_in_env rho1) fm (def_funs B B rhoc rhoc) rho2 i sig
+      | S k => fun_map_inv' k (occurs_free e \\ FromList xs) fm (def_funs B B rhoc rhoc) rho2 i sig
       end.
 
   Lemma fun_map_inv_eq k S fm rho1 rho2 n sig :
@@ -366,6 +409,7 @@ Section Inline_correct.
     intro; intros; eauto.
   Qed.
 
+  (* 
   Lemma occurs_free_in_env_set rho x v :
     occurs_free_in_env (M.set x v rho) \subset occurs_free_in_val v :|: occurs_free_in_env rho.
   Proof.
@@ -415,44 +459,83 @@ Section Inline_correct.
     - eapply occurs_free_in_env_get. simpl. rewrite M.gss. reflexivity. simpl. eassumption.
     - inv Hc. inv H. inv H.
   Qed.
-
+ 
+  
   Lemma sub_map_occurs_free_in_env rho1 rho2 :
     sub_map rho1 rho2 ->
     occurs_free_in_env rho1 \subset occurs_free_in_env rho2.
   Proof.
     intros Hs z Hin. inv Hin. destructAll.
     eapply Hs in H. do 4 eexists. split. eassumption. eassumption.
+  Qed. *)
+
+  Lemma add_fundefs_in fm f B ft xs e:
+    find_def f B = Some (ft, xs, e) -> 
+    (add_fundefs B fm) ! f = Some (ft, xs, e). 
+  Proof.
+    induction B.
+    - simpl. intros Hdef. destruct (M.elt_eq f v); subst.
+      + inv Hdef. simpl. rewrite M.gss. reflexivity.
+      + simpl. rewrite M.gso; eauto.
+    - intros H. inv H.
   Qed.
+
+  Lemma add_fundefs_not_in fm f B :
+    ~ f \in name_in_fundefs B -> 
+            (add_fundefs B fm) ! f = fm ! f.
+  Proof.
+    intros Hnin. induction B.
+    - simpl. rewrite M.gso. eapply IHB.
+      intros Hc. eapply Hnin. simpl. now right; eauto.
+      intros Hc. eapply Hnin. simpl. subst; eauto.
+    - reflexivity.
+  Qed.
+
+
+  Lemma occurs_free_fun_map_get f ft xs e (fm : fun_map) :
+    M.get f fm = Some (ft, xs, e) ->
+    occurs_free e \\ (FromList xs) \subset occurs_free_fun_map fm.
+  Proof.
+    intros Hget z Hin. do 4 eexists. split; eauto.
+  Qed.
+
+  Lemma occurs_free_fun_map_add_fundefs B fm :
+    occurs_free_fun_map (add_fundefs B fm) \subset occurs_free_fundefs B :|: name_in_fundefs B :|: occurs_free_fun_map fm.
+  Proof.
+    intros x [z Hin]. destructAll. destruct (Decidable_name_in_fundefs B). destruct (Dec z).
+    - edestruct name_in_fundefs_find_def_is_Some. eassumption. destructAll.
+      erewrite add_fundefs_in in H; eauto. inv H. left.
+      eapply find_def_correct in H1. eapply occurs_free_in_fun in H1.
+      inv H0. eapply H1 in H. inv H. contradiction. inv H0; eauto.
+    - right. rewrite add_fundefs_not_in in H. do 4 eexists; split; eauto.
+      eassumption.
+  Qed. 
+
 
   Lemma fun_map_inv_set_not_In_r k S fm rho1 rho2 i sig x x' v' : 
     fun_map_inv k S fm rho1 rho2 i sig ->
-    ~ x \in occurs_free_in_env rho1 ->
-    ~ x' \in image (apply_r sig) (occurs_free_in_env rho1) ->
+    ~ x \in occurs_free_fun_map fm ->
+    ~ x' \in image (apply_r sig) (occurs_free_fun_map fm) ->
     fun_map_inv k S fm rho1 (M.set x' v' rho2) i (M.set x x' sig).
   Proof.
     revert S fm rho1 rho2 i sig x x' v'. induction k using lt_wf_rec1; intros. intro; intros.
     edestruct H0; eauto.
     destructAll. split; [| split; [| split; [| split; [| split; [| split ]]]]]; eauto.
     - rewrite apply_r_set_f_eq. eapply preord_env_P_inj_set_extend_not_In_P_r. eassumption.
-      + intros Hc. eapply H1.   
-        eapply occurs_free_in_env_get. eassumption. simpl. now inv Hc; eauto.
+      + intros Hc. eapply H1. eapply occurs_free_fun_map_get; eassumption.
       + intros Hc. eapply H2. eapply image_monotonic; [| eassumption ]. 
-        eapply Included_trans; [| eapply occurs_free_in_env_get; eauto ]. simpl. sets.
-    - destruct k; eauto. rewrite <- fun_map_inv_eq in *. eapply H. omega. eassumption.
-      + intros Hc. eapply H1.
-        eapply sub_map_occurs_free_in_env. eassumption. eassumption.
-      + intros Hc. eapply H2. eapply image_monotonic; [| eassumption ].
-        eapply sub_map_occurs_free_in_env. eassumption.
+        eapply occurs_free_fun_map_get; eauto.
+    - destruct k; eauto. rewrite <- fun_map_inv_eq in *.
+      eapply H. omega. eassumption. eassumption. eassumption.
   Qed.                
     
   Lemma fun_map_inv_set k S fm rho1 rho2 i sig x v x' v' :
     fun_map_inv k S fm rho1 rho2 i sig ->
-    ~ x \in Dom_map rho1 :|: Dom_map fm :|: occurs_free_in_env rho1 ->
-    ~ x' \in image (apply_r sig) (occurs_free_in_env rho1) ->
-    occurs_free_in_val v \subset occurs_free_in_env rho1 ->
+    ~ x \in Dom_map rho1 :|: Dom_map fm :|: occurs_free_fun_map fm ->
+    ~ x' \in image (apply_r sig) (occurs_free_fun_map fm) ->
     fun_map_inv k (x |: S) fm (M.set x v rho1) (M.set x' v' rho2) i (M.set x x' sig).
   Proof.
-    intros Hinv Hnin Hnin' Hsub. intro; intros.
+    intros Hinv Hnin Hnin'. intro; intros.
     rewrite M.gso in *.
     2:{ intros Heq; subst. eapply Hnin. left. right. eexists; eauto. }
     inv H.
@@ -460,27 +543,19 @@ Section Inline_correct.
     - edestruct Hinv; eauto.
       destructAll. split; [| split; [| split; [| split; [| split; [| split ]]]]]; eauto.
       + rewrite apply_r_set_f_eq. eapply preord_env_P_inj_set_extend_not_In_P_r. eassumption.
-        intros Hc. eapply Hnin.  
-        right. eapply occurs_free_in_env_get. eassumption. simpl. now inv Hc; eauto.
-        intros Hc. eapply Hnin'. eapply image_monotonic; [| eassumption ]. 
-        eapply Included_trans; [| eapply occurs_free_in_env_get; eauto ]. simpl. sets.
+        intros Hc. eapply Hnin. right. eapply occurs_free_fun_map_get; eassumption. simpl.
+        intros Hc. eapply Hnin'. eapply image_monotonic; [| eassumption ].
+        eapply occurs_free_fun_map_get; eassumption.
       + eapply sub_map_trans. eassumption. eapply sub_map_set.
         intros Hc. eapply Hnin. left. left. eassumption.
-      + eapply Union_Disjoint_r; [| now sets ].
-        eapply Union_Disjoint_r; [ now sets | ]. eapply Disjoint_Included_r. eapply occurs_free_in_env_set.
-        rewrite Union_Same_set. sets. eassumption. 
-      + eapply Union_Disjoint_r; [| now sets ]. eapply Union_Disjoint_r; [| now sets ].
-        eapply Union_Disjoint_r; [ now sets | ]. eapply Disjoint_Included_r. eapply occurs_free_in_env_set.
-        rewrite Union_Same_set. sets. eassumption.         
       + destruct k; eauto. rewrite <- fun_map_inv_eq in *.
         eapply fun_map_inv_set_not_In_r. eapply fun_map_inv_antimon. eassumption.
-        * eapply Included_trans. eapply occurs_free_in_env_set. sets.
-        * intros Hc. eapply Hnin. right. eapply sub_map_occurs_free_in_env; eassumption.
-        * intros Hc. eapply Hnin'. eapply image_monotonic; [| eassumption ].
-          eapply sub_map_occurs_free_in_env; eassumption.
+        * reflexivity.
+        * intros Hc. eapply Hnin. right. eassumption.
+        * intros Hc. eapply Hnin'. eapply image_monotonic; [| eassumption ]. sets.
   Qed.
   
-
+(* 
   Lemma occurs_free_in_env_set_lists_not_In rho rho' xs vs :
     set_lists xs vs rho = Some rho' ->
     occurs_free_in_env rho' \subset \bigcup_(v in FromList vs) (occurs_free_in_val v) :|: occurs_free_in_env rho.
@@ -500,7 +575,7 @@ Section Inline_correct.
     intro; intros. rewrite <- H in H1. eauto.
     intro; intros. rewrite H in H1. eauto.
   Qed.
-
+*)
   Lemma Dom_map_set_lists {A} xs (vs : list A) rho rho' :
     set_lists xs vs rho = Some rho' ->
     Dom_map rho' <--> FromList xs :|: Dom_map rho.
@@ -539,7 +614,7 @@ Section Inline_correct.
   Lemma fun_map_inv_sig_extend_Disjoint k S fm rho1 rho2 i sig xs xs' :
     fun_map_inv k S fm rho1 rho2 i sig ->
 
-    Disjoint _ (FromList xs) (S :|: occurs_free_in_env rho1) ->    
+    Disjoint _ (FromList xs) (S :|: occurs_free_fun_map fm) ->    
     
     fun_map_inv k S fm rho1 rho2 i (set_list (combine xs xs') sig).
   Proof.
@@ -550,8 +625,7 @@ Section Inline_correct.
     - rewrite apply_r_set_list_f_eq. 
       eapply preord_env_P_inj_extend_lst_not_In_P_r. eassumption.
       eapply Disjoint_Included_r; [| eapply Hdis1 ].
-      eapply Included_Union_preserv_r. eapply Included_trans; [| eapply occurs_free_in_env_get; eauto ].
-      simpl; now sets.
+      eapply Included_Union_preserv_r. eapply occurs_free_fun_map_get; eauto.
     - eassumption.
     - eassumption.
     - eassumption.
@@ -559,28 +633,23 @@ Section Inline_correct.
       eassumption.
       eapply Disjoint_Included_r; [| eassumption ].
       eapply Included_Union_preserv_r. eapply Union_Included.
-      + reflexivity.
-      + eapply sub_map_occurs_free_in_env. eassumption.
+      + eapply occurs_free_fun_map_get; eauto.
+      + reflexivity. 
   Qed.
 
-  Lemma fun_map_inv_set_lists k S S' fm rho1 rho1' rho2 rho3 i sig xs xs' vs :
+  Lemma fun_map_inv_set_lists k S fm rho1 rho1' rho2 i sig xs xs' vs :
     fun_map_inv k S fm rho1 rho2 i sig ->
 
-    fun_map_inv k S' fm rho3 rho2 i sig ->
-    S \subset S' ->
-    \bigcup_(v in FromList vs) occurs_free_in_val v \subset occurs_free_in_env rho3 ->
-    sub_map rho1 rho3 ->
-    
     NoDup xs ->
-    Disjoint _ (FromList xs) (Dom_map rho1 :|: Dom_map fm :|: occurs_free_in_env rho3) ->    
+    Disjoint _ (FromList xs) (Dom_map rho1 :|: Dom_map fm :|: occurs_free_fun_map fm) ->    
     set_lists xs vs rho1 = Some rho1' ->
     
     fun_map_inv k (FromList xs :|: S) fm rho1' rho2 i (set_list (combine xs xs') sig).
   Proof.
-    revert S S' fm rho1 rho1' rho2 rho3 i sig xs xs' vs.
+    revert S fm rho1 rho1' rho2 i sig xs xs' vs.
     induction k using lt_wf_rec1;
-      intros S S' fm rho1 rho1' rho3 rho2 i sig xs xs' vs Hfm Hfm' Hsub Hsub' Hsm Hnd Hdis1 Hset.
-    intro; intros.
+      intros S fm rho1 rho1' rho2 i sig xs xs' vs Hfm Hnd Hdis1 Hset.
+    intro f; intros.
     destruct (Decidable_FromList xs). destruct (Dec f).
     - exfalso. eapply Hdis1. constructor. eassumption. left. right. eexists; eauto.
     - inv H0; try contradiction. erewrite <- set_lists_not_In in H2; [| eassumption | eassumption ].
@@ -588,55 +657,17 @@ Section Inline_correct.
       + rewrite apply_r_set_list_f_eq. 
         eapply preord_env_P_inj_extend_lst_not_In_P_r. eassumption.
         eapply Disjoint_Included_r; [| eapply Hdis1 ].
-        eapply Included_Union_preserv_r. eapply Included_trans; [| eapply occurs_free_in_env_get; eauto ].
-        simpl; now sets.
+        eapply Included_Union_preserv_r.  eapply occurs_free_fun_map_get; eauto.
       + eapply sub_map_trans. eassumption. eapply sub_map_set_lists. eassumption. eassumption.
         eapply Disjoint_Included_r; [| eapply Hdis1 ]. sets.
-      + edestruct Hfm'. eapply Hsub. eassumption. eassumption. eapply Hsm. eassumption.
-        destructAll.
-        eapply Union_Disjoint_r; [| now sets ]. eapply Union_Disjoint_r; [ now sets | ].
-        eapply Disjoint_Included_r. eapply occurs_free_in_env_set_lists_not_In. eassumption.
-        eapply Union_Disjoint_r; [| eapply Disjoint_Included_r; [| eapply H7]; now sets ].
-        eapply Disjoint_Included_r. eassumption. sets.
-      + edestruct Hfm'. eapply Hsub. eassumption. eassumption. eapply Hsm. eassumption.
-        destructAll.
-        eapply Union_Disjoint_r; [| now sets ]. eapply Union_Disjoint_r; [| now sets ]. eapply Union_Disjoint_r; [ now sets | ].
-        eapply Disjoint_Included_r. eapply occurs_free_in_env_set_lists_not_In. eassumption.
-        eapply Union_Disjoint_r; sets. eapply Disjoint_Included_r; [| eapply H8 ]. sets.
-      + destruct k; eauto.
-        edestruct Hfm'. now eauto. eassumption. eapply Hsm. eassumption. destructAll. 
-        rewrite <- fun_map_inv_eq in *. eapply fun_map_inv_sig_extend_Disjoint.
-        eapply fun_map_inv_antimon. eapply H15.
-        eapply Included_trans. eapply occurs_free_in_env_set_lists_not_In. eassumption.
-        eapply Union_Included. eassumption. eapply sub_map_occurs_free_in_env. eassumption.
-        eapply Disjoint_Included_r; [| eassumption ].
-        eapply Included_Union_preserv_r. eapply Union_Included.
-        * eapply Included_trans. eapply occurs_free_in_env_set_lists_not_In. eassumption.
-          eapply Union_Included. eassumption. eapply sub_map_occurs_free_in_env. eassumption.
-        * eapply sub_map_occurs_free_in_env. eassumption.
+      + eassumption.
+      + eassumption.
+      + destruct k; eauto. rewrite <- fun_map_inv_eq in *.
+        eapply fun_map_inv_sig_extend_Disjoint. eassumption.
+        apply Union_Disjoint_r; [| now sets ].
+        eapply Disjoint_Included_r. eapply occurs_free_fun_map_get. eassumption. sets.
   Qed.
   
-  Lemma add_fundefs_in fm f B ft xs e:
-    find_def f B = Some (ft, xs, e) -> 
-    (add_fundefs B fm) ! f = Some (ft, xs, e). 
-  Proof.
-    induction B.
-    - simpl. intros Hdef. destruct (M.elt_eq f v); subst.
-      + inv Hdef. simpl. rewrite M.gss. reflexivity.
-      + simpl. rewrite M.gso; eauto.
-    - intros H. inv H.
-  Qed.
-
-  Lemma add_fundefs_not_in fm f B :
-    ~ f \in name_in_fundefs B -> 
-    (add_fundefs B fm) ! f = fm ! f.
-  Proof.
-    intros Hnin. induction B.
-    - simpl. rewrite M.gso. eapply IHB.
-      intros Hc. eapply Hnin. simpl. now right; eauto.
-      intros Hc. eapply Hnin. simpl. subst; eauto.
-    - reflexivity.
-  Qed.
 
   Lemma Dom_map_add_fundefs fm B :
     Dom_map (add_fundefs B fm) <--> name_in_fundefs B :|: Dom_map fm.
@@ -663,42 +694,54 @@ Section Inline_correct.
                      (def_funs B1 B1 rho1 rho1) (def_funs B2 B2 rho2 rho2) ->
 
     unique_bindings_fundefs B1 ->
-    occurs_free_fundefs B1 :|: occurs_free_in_env rho1 \subset S ->
+    occurs_free_fundefs B1 \subset S ->
     
-    Disjoint _ (name_in_fundefs B1) (S :|: Dom_map rho1 :|: occurs_free_in_env rho1) ->
-
+    Disjoint _ (bound_var_fundefs B1) (S :|: Dom_map rho1 :|: occurs_free_fun_map fm :|: bound_var_fun_map fm) ->
+    Disjoint _ (name_in_fundefs B2) (image (apply_r sig) (occurs_free_fun_map fm)) ->
+    
     fun_map_inv k (name_in_fundefs B1 :|: S) (add_fundefs B1 fm) (def_funs B1 B1 rho1 rho1) (def_funs B2 B2 rho2 rho2) i
                 (set_list (combine (all_fun_name B1) (all_fun_name B2)) sig).
   Proof.
     revert S fm rho1 rho2 i sig B1 B2. induction k as [k IHk] using lt_wf_rec1.
-    intros S fm rho1 rho2 i sig B1 B2 Hf Hrel Hun Hsub Hdis.
-    intros f ft xs e rhoc B' f' HSin Heq1 Heq2.   
+    intros S fm rho1 rho2 i sig B1 B2 Hf Hrel Hun Hsub Hdis Hdis'.
+    intros f ft xs e rhoc B' f' HSin Heq1 Heq2.
     destruct (Decidable_name_in_fundefs B1) as [Dec]. destruct (Dec f).
     - rewrite def_funs_eq in Heq2; eauto. inv Heq2.
       edestruct name_in_fundefs_find_def_is_Some. eassumption. destructAll.
       erewrite add_fundefs_in in Heq1; [| eassumption ]. inv Heq1. split; eauto.
       split; eauto. split; [| split; [| split; [| split ]]].
-      + eassumption.
+      + eapply preord_env_P_inj_antimon. eassumption. eapply Setminus_Included_Included_Union.
+        eapply Included_trans. eapply occurs_free_in_fun. eapply find_def_correct. eassumption. sets.
       + eapply sub_map_refl.
-      + admit. (* seems OK *)
+      + sets. admit. (* seems OK *)
       + rewrite Dom_map_add_fundefs.
         admit. (* seems OK, add assump *)
       + destruct k; eauto. rewrite <- fun_map_inv_eq. eapply fun_map_inv_antimon. eapply IHk.
         omega. eapply fun_map_inv_mon. eassumption. omega. eassumption. eassumption.
-        eassumption. now sets. 
-        eapply Included_trans. eapply occurs_free_in_env_def_funs.
-        rewrite (Union_commut (occurs_free_fundefs _)). rewrite <- Union_assoc.
-        eapply Union_Included. now sets. eapply Included_trans. eassumption. sets.
+        eassumption. eassumption. now sets. eapply Setminus_Included_Included_Union.
+        eapply Included_trans. eapply occurs_free_in_fun. eapply find_def_correct. eassumption.
+        sets. 
     - rewrite def_funs_neq in Heq2; eauto.
-      rewrite add_fundefs_not_in in Heq1; [| eassumption ]. inv HSin. contradiction. 
-      edestruct Hf. eassumption. eassumption. eassumption. destructAll. split; eauto. split; eauto. 
-      split; [| split; [| split; [| split ]]].
+      rewrite add_fundefs_not_in in Heq1; [| eassumption ]. inv HSin. contradiction.
+      edestruct Hf. eassumption. eassumption. eassumption. destructAll. split; eauto. split; eauto.
+      split; [| split; [| split; [| split ]]]; eauto.
       + eapply preord_env_P_inj_def_funs_neq_r.
-
         rewrite apply_r_set_list_f_eq. eapply preord_env_P_inj_extend_lst_not_In_P_r.
-        eassumption. admit. admit. (* I think OK *)
-      + eapply sub_map_trans. eassumption. eapply sub_map_def_funs. sets.
-      + admit. (* I think OK *)
+        eassumption.
+        * rewrite <- Same_set_all_fun_name.
+          eapply Disjoint_Included; [| | eapply Hdis ]. eapply Included_trans. eapply occurs_free_fun_map_get. eassumption.
+          sets. eapply name_in_fundefs_bound_var_fundefs.
+        * rewrite apply_r_set_list_f_eq. eapply Disjoint_Included_l.
+          intros x Hc. destruct Hc. destructAll.
+          rewrite extend_lst_gso. eapply In_image. eassumption.
+          rewrite <- Same_set_all_fun_name. intros Hc. eapply Hdis. constructor.
+          eapply name_in_fundefs_bound_var_fundefs. eassumption.           
+          right. eapply occurs_free_fun_map_get. eassumption. eassumption.
+          eapply Disjoint_sym. eapply Disjoint_Included; [| | eapply Hdis' ]. eapply image_monotonic.
+           eapply occurs_free_fun_map_get. eassumption. reflexivity. 
+      + eapply sub_map_trans. eassumption. eapply sub_map_def_funs.
+        eapply Disjoint_Included; [| | eapply Hdis ]; sets. eapply name_in_fundefs_bound_var_fundefs. 
+      + rewrite Dom_mapadmit. (* I think OK *)
       + admit.
       + destruct k; eauto. rewrite <- fun_map_inv_eq in *.
  
@@ -707,18 +750,32 @@ Section Inline_correct.
  
   Lemma fun_map_inv_add_fundefs_Disjoint k S fm rho1 rho2 i sig B1 B2 :
     fun_map_inv k S fm rho1 rho2 i sig ->
-    Disjoint _ (name_in_fundefs B1) (S :|: occurs_free_in_env rho1) ->
+
+    Disjoint _ (name_in_fundefs B1) (S :|: occurs_free_fun_map fm) ->
+    Disjoint _ (name_in_fundefs B2) (image (apply_r sig) (occurs_free_fun_map fm)) ->
+
     fun_map_inv k S (add_fundefs B1 fm) rho1 (def_funs B2 B2 rho2 rho2) i
                 (set_list (combine (all_fun_name B1) (all_fun_name B2)) sig).
   Proof.
     revert S fm rho1 rho2 i sig B1 B2; induction k using lt_wf_rec1; intros.
-    intro; intros. rewrite add_fundefs_not_in in H3.
+    intro; intros. rewrite add_fundefs_not_in in H4.
     edestruct H0; eauto. destructAll.
     repeat (split; [ now eauto |]). split; [| split; [| split; [| split ]]].
-    - admit.
+    - eapply preord_env_P_inj_def_funs_neq_r.
+      rewrite apply_r_set_list_f_eq. eapply preord_env_P_inj_extend_lst_not_In_P_r.
+      eassumption. rewrite <- Same_set_all_fun_name.
+      eapply Disjoint_Included_r. eapply occurs_free_fun_map_get. eassumption. sets.
+      rewrite apply_r_set_list_f_eq. eapply Disjoint_Included_l.
+      intros x Hc. destruct Hc. destructAll.
+      rewrite extend_lst_gso. eapply In_image. eassumption.
+      rewrite <- Same_set_all_fun_name. intros Hc. eapply H1. constructor. eassumption.
+      right. eapply occurs_free_fun_map_get. eassumption. eassumption.
+      eapply Disjoint_sym. eapply Disjoint_Included_r; [| eassumption ]. eapply image_monotonic.
+      eapply occurs_free_fun_map_get. eassumption. 
+    - eassumption.
+    - eassumption. preoradmit.
     - eassumption.
     - sets.
-    - 
   (*   - destruct k; eauto. rewrite <- fun_map_inv_eq in *. eapply H. *)
   (*     + omega. *)
   (*     + eassumption. *)
@@ -742,11 +799,8 @@ Section Inline_correct.
       fm ! f = Some (ft, xs, e) ->
       unique_bindings e /\
       NoDup xs /\
-      Disjoint _ (bound_var e) (occurs_free e :|: Dom_map fm) /\
-      Disjoint _ F (bound_var e :|: image (apply_r sig) (occurs_free e)).
-
-  Definition occurs_free_fun_map (fm : fun_map) : Ensemble var :=
-    fun v => exists f ft xs e, fm ! f = Some (ft, xs, e) /\ v \in (occurs_free e \\ FromList xs).
+      Disjoint _ (bound_var e) (occurs_free e :|: Dom_map fm :|: occurs_free_fun_map fm) /\
+      Disjoint _ F (bound_var e :|: image (apply_r sig) (occurs_free e :|: occurs_free_fun_map fm)).
 
   Lemma fun_map_vars_set fm F sig x v :
     fun_map_vars fm F sig ->
@@ -764,65 +818,89 @@ Section Inline_correct.
     induction B; simpl; sets.
     rewrite Dom_map_set. rewrite IHB. sets.
   Qed.
+
+  Lemma apply_r_list_eq xs ys sig :
+    NoDup xs ->
+    length xs = length ys ->
+    apply_r_list (set_list (combine xs ys) sig) xs = ys.
+  Proof.
+    revert ys sig; induction xs; intros ys sig Hnd Hlen.
+    - simpl. destruct ys; eauto. inv Hlen.
+    - destruct ys; inv Hlen. inv Hnd.
+      simpl. unfold apply_r. rewrite M.gss. f_equal.
+      erewrite eq_P_apply_r_list. eapply IHxs. eassumption. eassumption.
+      eapply eq_env_P_set_not_in_P_l. eapply eq_env_P_refl. eassumption.
+  Qed.
+
+  Lemma NoDup_all_fun_name B :
+    unique_bindings_fundefs B ->
+    NoDup (all_fun_name B).
+  Proof.
+    induction B; intros Hc; inv Hc.
+    - simpl. constructor; eauto.
+      intros Hc. eapply Same_set_all_fun_name in Hc. eapply H5.
+      eapply name_in_fundefs_bound_var_fundefs. eassumption.
+    - constructor.
+  Qed.
+    
     
   Opaque preord_exp'.
   
   Lemma inline_correct_mut d : 
-    (forall e sig fm st S,
-        unique_bindings e ->
-        Disjoint _ (bound_var e) (occurs_free e :|: Dom_map fm) ->    
-        Disjoint _ S (bound_var e :|: image (apply_r sig) (occurs_free e)) ->        
-        fun_map_vars fm S sig ->        
+    (forall e sig fm st S
+            (Hun : unique_bindings e)
+            (Hdis1 : Disjoint _ (bound_var e) (occurs_free e :|: occurs_free_fun_map fm :|: Dom_map fm))    
+            (Hdis2: Disjoint _ S (bound_var e :|: image (apply_r sig) (occurs_free e :|: occurs_free_fun_map fm)))
+            (Hfm : fun_map_vars fm S sig),
         {{ fun _ s => fresh S (next_var (fst s)) }}
           beta_contract St IH d e sig fm st
-        {{ fun _ _ e' s' =>
-             fresh S (next_var (fst s')) /\
+        {{ fun _ s e' s' =>
+             fresh S (next_var (fst s')) /\ next_var (fst s) <= next_var (fst s') /\
              unique_bindings e' /\
              occurs_free e' \subset image (apply_r sig) (occurs_free e :|: occurs_free_fun_map fm) /\
-             bound_var e' \subset S /\
+             bound_var e' \subset (Range (next_var (fst s)) (next_var (fst s')))  /\
              (forall k rho1 rho2,
                  preord_env_P_inj cenv PG (occurs_free e) k (apply_r sig) rho1 rho2 ->
-                 Disjoint _ (bound_var e) (occurs_free_in_env rho1 :|: Dom_map rho1) ->
-                 Disjoint _ S (image (apply_r sig) (occurs_free_in_env rho1)) ->
-                 fun_map_inv d (occurs_free e :|: occurs_free_in_env rho1) fm rho1 rho2 k sig ->
+                 Disjoint _ (bound_var e) (Dom_map rho1) ->
+                 fun_map_inv d (occurs_free e) fm rho1 rho2 k sig ->
                  preord_exp cenv P1 PG k (e, rho1) (e', rho2)) }} ) /\ 
 
-    (forall B sig sig0 fm st S,
-        unique_bindings_fundefs B ->
-        Disjoint _ (bound_var_fundefs B) (occurs_free_fundefs B :|: Dom_map fm) ->    
-        Disjoint _ S (bound_var_fundefs B :|: image (apply_r sig) (occurs_free_fundefs B)) ->
-        fun_map_vars fm S sig ->        
+    (forall B sig sig0 fm st S
+            (Hun : unique_bindings_fundefs B)
+            (Hdis1 : Disjoint _ (bound_var_fundefs B) ((occurs_free_fundefs B :|: occurs_free_fun_map fm :|: Dom_map fm) \\ name_in_fundefs B))
+            (Hdis2 : Disjoint _ S (bound_var_fundefs B :|: image (apply_r sig) (occurs_free_fundefs B :|: occurs_free_fun_map fm)))
+            (Hfm : fun_map_vars fm S sig), 
         {{ fun _ s => fresh S (next_var (fst s)) }}
-          beta_contract_fundefs St IH d sig sig0 fm B st
-        {{ fun _ _ B' s' =>
-             fresh S (next_var (fst s')) /\
+          beta_contract_fundefs St IH d sig0 sig fm B st
+        {{ fun _ s B' s' =>
+             fresh S (next_var (fst s')) /\ next_var (fst s) <= next_var (fst s') /\
              unique_bindings_fundefs B' /\
              occurs_free_fundefs B' \subset image (apply_r sig) (occurs_free_fundefs B :|: occurs_free_fun_map fm) /\
-             bound_var_fundefs B' \subset S /\
+             bound_var_fundefs B' \subset (Range (next_var (fst s)) (next_var (fst s'))) /\
              all_fun_name B' = apply_r_list sig (all_fun_name B) /\
              (forall f xs ft e1,
-                 find_def f B = Some (xs, ft, e1) ->
+                 find_def f B = Some (ft, xs, e1) ->
                  exists xs' e2,
-                   find_def (apply_r sig f) B = Some (xs', ft, e2) /\
+                   find_def (apply_r sig f) B' = Some (ft, xs', e2) /\
+                   length xs = length xs' /\ NoDup xs' /\ FromList xs' \subset S /\
                    (forall rho1 rho2 k,
-                       preord_env_P_inj cenv PG (occurs_free_fundefs B) k (apply_r sig) rho1 rho2 ->
-                       Disjoint _ (bound_var e1) (occurs_free_in_env rho1 :|: Dom_map rho1) ->
-                       Disjoint _ S (image (apply_r sig) (occurs_free_in_env rho1)) ->
-                       fun_map_inv d (occurs_free_fundefs B :|: occurs_free_in_env rho1) fm rho1 rho2 k sig ->
-                       preord_exp cenv P1 PG k (e1, rho1) (e2, rho2)))}}).
+                       preord_env_P_inj cenv PG (occurs_free_fundefs B) k (apply_r sig <{ xs ~> xs' }>) rho1 rho2 ->
+                       Disjoint _ (bound_var e1) (Dom_map rho1) ->
+                       fun_map_inv d (occurs_free_fundefs B) fm rho1 rho2 k sig ->
+                       preord_exp cenv P1 PG k (e1, rho1) (e2, rho2))) }}).
 
   Proof.
-    revert e sig fm st S. induction d as [d IHd] using lt_wf_rec1.
-    induction e using exp_ind'; intros sig fm st S Hun Hdis1 Hdis2 Hfm; inv Hun; rewrite beta_contract_eq.
+    induction d as [d IHd] using lt_wf_rec1.
+    exp_defs_induction IHe IHl IHB; intros; inv Hun; try rewrite beta_contract_eq.
     - (* constr *)
-      eapply bind_triple. now eapply get_name_fresh. 
-      intros x w1. eapply pre_curry_l. intros Hinx.
-      eapply bind_triple. eapply IHe with (S := S \\ [set x]).
+      eapply bind_triple. eapply pre_transfer_r. now eapply get_name_fresh. 
+      intros x w1. simpl. eapply pre_curry_l. intros Hf. 
+      eapply bind_triple. eapply frame_rule. eapply frame_rule. eapply IHe with (S := S \\ [set x]).
       + eassumption.
       + repeat normalize_bound_var_in_ctx. repeat normalize_occurs_free_in_ctx.
         eapply Disjoint_Included_r. eapply Included_Union_Setminus with (s2 := [set v]). tci.
-        eapply Union_Disjoint_r. eapply Disjoint_Included; [| | eapply Hdis1].
-        rewrite Setminus_Union_distr. now sets. now sets.
+        rewrite !Setminus_Union_distr. eapply Union_Disjoint_r.
+        now eapply Disjoint_Included; [| | eapply Hdis1 ]; sets.
         eapply Disjoint_Singleton_r. eassumption.
       + eapply Disjoint_Included_r.
         eapply Included_Union_compat. reflexivity.
@@ -831,23 +909,27 @@ Section Inline_correct.
         eapply Union_Disjoint_r. now sets.
         eapply Union_Disjoint_r. now sets.
         eapply Disjoint_Included; [| | eapply Hdis2 ].
-        rewrite !image_Union. now xsets. now sets.
+        rewrite Setminus_Union_distr. rewrite !image_Union. now xsets. now sets.
       + eapply fun_map_vars_set. eassumption.
       + intros e' w2. eapply return_triple.
-        intros _ st'. intros [Hf [Hun [Hsub [Hsub' Hsem]]]].
-        split; [| split; [| split; [| split ]]].
+        intros _ st'. intros [Hf1 [Hf2 [Hf3 [Hf4 [Hun [Hsub [Hsub' Hsem]]]]]]].
+        split; [| split; [| split; [| split; [| split ]]]].
         * eapply fresh_monotonic;[| eassumption ]. sets.
-        * constructor.
-          intros Hc. eapply Hsub' in Hc. now inv Hc; eauto. eassumption. 
+        * zify; omega.
+        * constructor; [| eassumption ].
+          intros Hc. eapply Hsub' in Hc. eapply Disjoint_Range; [| constructor; [ eapply Hf1 | eapply Hc ]].
+          reflexivity.
         * repeat normalize_occurs_free. rewrite !image_Union.
           rewrite <- FromList_apply_list. rewrite <- !Union_assoc. eapply Included_Union_compat. reflexivity. 
           eapply Included_trans. eapply Included_Setminus_compat.
           eapply Included_trans. eassumption. now eapply image_apply_r_set. reflexivity.
           rewrite !Setminus_Union_distr. rewrite Setminus_Same_set_Empty_set. normalize_sets.
           rewrite image_Union. sets.
-        * normalize_bound_var. eapply Union_Included. eapply Included_trans. eassumption. now sets.
-          eapply Singleton_Included. eassumption.
-        * intros r1 r2 k Henv Hdis Hdis' Hfm'. eapply preord_exp_const_compat.
+        * normalize_bound_var. eapply Union_Included. eapply Included_trans. eassumption.
+          eapply Range_Subset. zify; omega. reflexivity.
+          eapply Included_trans. eapply Singleton_Included. eassumption. eapply Range_Subset. reflexivity.
+          zify; omega.
+        * intros r1 r2 k Henv Hdis Hfm'. eapply preord_exp_const_compat.
           eassumption. eassumption.
           eapply Forall2_preord_var_env_map. eassumption. normalize_occurs_free. now sets.          
           intros. eapply Hsem. 
@@ -856,29 +938,31 @@ Section Inline_correct.
              omega. normalize_occurs_free. sets.
           -- rewrite preord_val_eq. split. reflexivity.
              eapply Forall2_Forall2_asym_included. eassumption.
-          -- intros Hc. eapply Hdis2. constructor. eassumption.
-             right. normalize_occurs_free. rewrite image_Union. right. eassumption.
+          -- intros Hc. eapply Hdis2. constructor. eapply Hf. eapply Hf1. 
+             right. normalize_occurs_free. rewrite !image_Union. left. right. eassumption.
           -- repeat normalize_bound_var_in_ctx. rewrite Dom_map_set.
              eapply Union_Disjoint_r.
-             ++ eapply Disjoint_Included_r. eapply occurs_free_in_env_set. simpl. normalize_sets.
-                eapply Disjoint_Included; [| | eapply Hdis]; sets.
-             ++ eapply Union_Disjoint_r.
-                ** eapply Disjoint_Singleton_r. eassumption.
-                ** eapply Disjoint_Included; [| | eapply Hdis]; sets.
-          -- eapply Disjoint_Included_r.
-             eapply Included_trans. eapply image_monotonic. eapply occurs_free_in_env_set. simpl. repeat normalize_sets.
-             now eapply image_apply_r_set.
-             eapply Union_Disjoint_r. now sets. sets. 
+             ++ eapply Disjoint_Singleton_r. eassumption.
+               (* eapply Disjoint_Included_r. eapply occurs_free_in_env_set. simpl. normalize_sets. *)
+               (*  eapply Disjoint_Included; [| | eapply Hdis]; sets. *)
+             ++ sets.
+                (* eapply Union_Disjoint_r. *)
+                (* ** eapply Disjoint_Singleton_r. eassumption. *)
+                (* ** eapply Disjoint_Included; [| | eapply Hdis]; sets. *)
+            (* eapply Disjoint_Included_r. *)
+            (*  eapply Included_trans. eapply image_monotonic. eapply occurs_free_in_env_set. simpl. repeat normalize_sets. *)
+            (*  now eapply image_apply_r_set. *)
+            (*  eapply Union_Disjoint_r. now sets. sets.  *)
           -- eapply fun_map_inv_antimon. eapply fun_map_inv_set. eapply fun_map_inv_i_mon. eassumption. omega.
              intros Hc. inv Hc. inv H2.
-             ++ eapply Hdis. normalize_bound_var. constructor. now right. now right; eauto.
+             ++ eapply Hdis. normalize_bound_var. constructor. now right. eassumption.
              ++ eapply Hdis1. constructor. normalize_bound_var. now right. now right; eauto.
-             ++ eapply Hdis. normalize_bound_var. constructor. now right. now left; eauto.
-             ++ intros Hc. eapply Hdis'. constructor; eassumption.
-             ++ simpl. sets.
+             ++ eapply Hdis1. normalize_bound_var. constructor. now right. now left; right.
+             ++ intros Hc. eapply Hdis2. constructor; try eassumption.
+                eapply fresh_Range; [| eassumption ]. eassumption. rewrite image_Union. eauto.
              ++ normalize_occurs_free. rewrite !Union_assoc. rewrite Union_Setminus_Included; sets; tci.
-                eapply Union_Included. now sets. eapply Included_trans. eapply occurs_free_in_env_set.
-                simpl. sets.
+                (* eapply Union_Included. now sets. eapply Included_trans. eapply occurs_free_in_env_set. *)
+                (* simpl. sets. *)
     - (* Ecase [] *)
       admit.
     - (* Ecase (_ :: _) *)
@@ -887,46 +971,163 @@ Section Inline_correct.
       admit.
     - (* Eletapp *)
       admit.
-    - (* Efun *)
+    - (* Efun *) 
       simpl. destruct (update_funDef St IH f2 sig st). 
-      eapply bind_triple. now eapply get_names_lst_fresh. intros xs w.
-      eapply pre_curry_l. intros Hinx.
-      eapply pre_curry_l. intros Hnd. eapply bind_triple. admit.
-      intros fds' w'. eapply bind_triple. eapply IHe.
-      + eassumption.
-      + rewrite Dom_map_add_fundefs.
-        rewrite Union_Included_Union_Setminus with (s3 := name_in_fundefs f2); [| now tci | now sets ]. 
-        rewrite (Union_commut (name_in_fundefs f2)). rewrite Union_assoc.
-        eapply Union_Disjoint_r.
-        * repeat normalize_bound_var_in_ctx. repeat normalize_occurs_free_in_ctx.
-          eapply Disjoint_Included; [| | eapply Hdis1 ]; now sets.
-        * eapply Disjoint_Included_r; [| eassumption ].
-          eapply name_in_fundefs_bound_var_fundefs.
-      + admit.
-      + admit.
-      + intros e' w''. eapply return_triple. intros _ w''' Hyp. destructAll.
-        split; [| split; [| split; [| split ]]].
-        * admit.
-        * admit.
-        * admit.
-        * admit.
-        * intros k rho1 rho2 Henv Hdis Hdis' Hfm'. eapply preord_exp_fun_compat.
-          eassumption. eassumption.
-          eapply H6.
-          -- admit.
-          -- admit.
-          -- admit.
-          -- admit. 
-      admit.
+      eapply bind_triple. eapply pre_transfer_r. now eapply get_names_lst_fresh. intros xs w. simpl.
+      eapply pre_curry_l. intros Hf. eapply pre_curry_l. intros Hnd.  eapply pre_curry_l. intros Hlen.
+      eapply bind_triple. 
+      { do 2 eapply frame_rule. eapply IHB with (S := S \\ FromList xs).
+        - eassumption.
+        - repeat normalize_occurs_free_in_ctx. repeat normalize_bound_var_in_ctx.
+          eapply Disjoint_Included; [| | eapply Hdis1 ]; try now sets.
+          rewrite !Setminus_Union_distr. eapply Union_Included. eapply Union_Included. now sets.
+          eapply Included_trans. eapply Included_Setminus_compat. eapply occurs_free_fun_map_add_fundefs. reflexivity.
+          rewrite Setminus_Union_distr. now sets.
+          rewrite Dom_map_add_fundefs. rewrite Setminus_Union_distr. now sets.
+        - repeat normalize_occurs_free_in_ctx. repeat normalize_bound_var_in_ctx. 
+          rewrite image_Union in Hdis2. eapply Union_Disjoint_r. now sets.
+          eapply Disjoint_Included_r. eapply image_apply_r_set_list. now eauto.
+          eapply Union_Disjoint_r. now sets.
+          rewrite <- Same_set_all_fun_name. rewrite Setminus_Union_distr. rewrite image_Union. eapply Union_Disjoint_r.
+          now xsets.
+          eapply Disjoint_Included_r. eapply image_monotonic. eapply Included_Setminus_compat. eapply occurs_free_fun_map_add_fundefs. reflexivity.
+          rewrite !Setminus_Union_distr. rewrite Setminus_Same_set_Empty_set. repeat normalize_sets. rewrite image_Union. xsets. 
+        - admit. (* fun_map_vars *)
+          (* fun_map_vars (add_fundefs f2 fm) (S \\ FromList xs) *)
+          (*              (set_list (combine (all_fun_name f2) xs) sig) *)
+      }
+      intros fds' w'. simpl.
+      eapply pre_curry_l. intros Hsub. eapply pre_curry_l. intros Hr. 
+      eapply bind_triple.
+      { eapply pre_strenghtening.
+        2:{ eapply frame_rule. eapply IHe with (S := S \\ FromList xs).
+            + eassumption.
+            + rewrite Dom_map_add_fundefs.
+              rewrite Union_Included_Union_Setminus with (s3 := name_in_fundefs f2); [| now tci | now sets ]. 
+              rewrite (Union_commut (name_in_fundefs f2)). rewrite Union_assoc.
+              eapply Union_Disjoint_r.
+              * repeat normalize_bound_var_in_ctx. repeat normalize_occurs_free_in_ctx. rewrite Setminus_Union_distr. 
+                eapply Disjoint_Included; [| | eapply Hdis1 ]. eapply Union_Included. eapply Union_Included. now sets.
+                eapply Setminus_Included_Included_Union. eapply Included_trans. eapply occurs_free_fun_map_add_fundefs. now xsets.
+                now sets. now sets.
+              * eapply Disjoint_Included_r; [| eassumption ].
+                eapply name_in_fundefs_bound_var_fundefs.
+            + repeat normalize_bound_var_in_ctx. repeat normalize_occurs_free_in_ctx.
+              eapply Union_Disjoint_r. now sets. eapply Disjoint_Included_r.
+              eapply image_apply_r_set_list. now eauto.
+              rewrite image_Union in Hdis2. eapply Union_Disjoint_r. now xsets.
+              rewrite <- Same_set_all_fun_name. rewrite Setminus_Union_distr. rewrite image_Union.
+              eapply Union_Disjoint_r. now xsets.
+              eapply Disjoint_Included_r. eapply image_monotonic. eapply Included_Setminus_compat. eapply occurs_free_fun_map_add_fundefs. reflexivity.
+              rewrite !Setminus_Union_distr. rewrite image_Union. xsets.
+            + admit. (* fun_map vars *)
+              (*   fun_map_vars (add_fundefs f2 fm) (S \\ FromList xs)
+                   (set_list (combine (all_fun_name f2) xs) sig) *) 
+        }  
+      simpl. intros u w1 [Hyp Hyp']. split. eapply Hyp'. eassumption. }
+      intros e' w''. eapply return_triple. intros _ w''' Hyp. destructAll.
+      assert (Hnd' := NoDup_all_fun_name _ H2).
+      split; [| split; [| split; [| split; [| split ]]]].
+      * eapply fresh_monotonic; [| eassumption ]. sets.
+      * zify; omega. 
+      * constructor. eassumption. eassumption.
+        eapply Disjoint_Included. eassumption. eassumption.
+        eapply Disjoint_sym. eapply Disjoint_Range. reflexivity.
+      * repeat normalize_occurs_free. eapply Union_Included.
+        -- eapply Included_trans. eapply Included_Setminus. eapply Disjoint_sym.
+           eapply occurs_free_fundefs_name_in_fundefs_Disjoint. reflexivity.
+           eapply Setminus_Included_Included_Union. eapply Included_trans. eassumption.
+           eapply Included_trans. eapply image_apply_r_set_list. now eauto.
+           rewrite (Same_set_all_fun_name fds'). rewrite H12.
+           rewrite apply_r_list_eq; eauto. eapply Union_Included. now sets.
+           eapply Included_Union_preserv_l. rewrite <- Same_set_all_fun_name.
+           rewrite Setminus_Union_distr. rewrite !image_Union. eapply Union_Included. now sets.
+           eapply Included_trans. eapply image_monotonic. eapply Included_Setminus_compat.
+           eapply occurs_free_fun_map_add_fundefs. reflexivity.
+           rewrite !Setminus_Union_distr, Setminus_Same_set_Empty_set. repeat normalize_sets.
+           rewrite image_Union. now xsets.
+        -- eapply Included_trans. eapply Included_Setminus_compat. eassumption. reflexivity.
+           eapply Setminus_Included_Included_Union. 
+           eapply Included_trans. eapply image_apply_r_set_list. now eauto.
+           rewrite (Same_set_all_fun_name fds'). rewrite H12.
+           rewrite apply_r_list_eq; eauto. eapply Union_Included. now sets.
+           eapply Included_Union_preserv_l. rewrite <- Same_set_all_fun_name.
+           rewrite Setminus_Union_distr. rewrite !image_Union. eapply Union_Included. now sets.
+           eapply Included_trans. eapply image_monotonic. eapply Included_Setminus_compat.
+           eapply occurs_free_fun_map_add_fundefs. reflexivity.
+           rewrite !Setminus_Union_distr, Setminus_Same_set_Empty_set. repeat normalize_sets.
+           rewrite image_Union. now xsets.
+      * normalize_bound_var. eapply Union_Included.
+        -- eapply Included_trans. eassumption. eapply Range_Subset. eassumption. zify; omega.
+        -- eapply Included_trans. eassumption. eapply Range_Subset. zify; omega. reflexivity.
+      * intros k rho1 rho2 Henv Hdis Hfm'. eapply preord_exp_fun_compat.
+        eassumption. eassumption. eapply H8.
+        -- { eapply preord_env_P_inj_antimon with (S2 := name_in_fundefs f2 :|: occurs_free (Efun f2 e)).
+             2:{ normalize_occurs_free. rewrite !Union_assoc. rewrite Union_Setminus_Included; sets. tci. }
+             assert (Hi : (k - 1 <= k)%nat) by omega.
+             revert Hi. generalize (k - 1)%nat as i. intros i Hi. induction i as [i IHi] using lt_wf_rec1. 
+             assert (Hseq :  apply_r_list (set_list (combine (all_fun_name f2) xs) sig) (all_fun_name f2) = xs).
+             { rewrite apply_r_list_eq. reflexivity. now eauto. now eauto. }
+             
+             intros x HIn v Hgetx. destruct (Decidable_name_in_fundefs f2). destruct (Dec x).
+             - rewrite def_funs_eq in Hgetx; [| now eauto ]. inv Hgetx. eexists. split.
+               + rewrite def_funs_eq. reflexivity. eapply Same_set_all_fun_name. 
+                 rewrite H12. rewrite FromList_apply_list. eapply In_image.
+                 rewrite <- Same_set_all_fun_name. eassumption.
+               + rewrite preord_val_eq. intros vs1 vs2 j t1 ys1 e2 rho1' Hlen' Hfind Hset.
+                 edestruct H13. eassumption. destructAll.
+                 edestruct set_lists_length2 with (xs2 := x0) (vs2 := vs2) (rho' := def_funs fds' fds' rho2 rho2). 
+                 now eauto. eassumption. now eauto. do 3 eexists. split. eassumption. split. now eauto. 
+                 intros Hlt Hvs. eapply preord_exp_post_monotonic. eassumption. eapply H18.
+                 * eapply preord_env_P_inj_set_lists_alt; [| eassumption | | | | | now eauto | now eauto ]. 
+                   -- eapply preord_env_P_inj_antimon. eapply IHi. eassumption. omega.
+                      normalize_occurs_free. sets.
+                   -- eapply unique_bindings_fun_in_fundefs. eapply find_def_correct. eassumption.
+                      eassumption.
+                   -- eassumption.
+                   -- eassumption.
+                   -- eapply Disjoint_Included_r. eassumption.
+                      eapply Disjoint_Included_l. eapply image_apply_r_set_list. now eauto.
+                      eapply Union_Disjoint_l. now sets. rewrite <- Same_set_all_fun_name.
+                      eapply Disjoint_sym. eapply Disjoint_Included; [| | eapply Hdis2 ].
+                      normalize_occurs_free. now xsets. now sets.
+                 * rewrite Dom_map_set_lists; [| now eauto ]. rewrite Dom_map_def_funs.
+                   eapply Union_Disjoint_r. eapply unique_bindings_fun_in_fundefs. eapply find_def_correct. eassumption. eassumption.
+                   eapply Union_Disjoint_r. eapply unique_bindings_fun_in_fundefs. eapply find_def_correct. eassumption. eassumption.
+                   eapply Disjoint_Included_l; [| eapply Hdis ]. normalize_bound_var. eapply Included_Union_preserv_l.
+                   eapply Included_trans; [| eapply fun_in_fundefs_bound_var_fundefs ]; [| eapply find_def_correct; eassumption ]. sets.
+                 * (* eapply fun_map_inv_antimon. eapply fun_map_inv_set_lists. *)
+                   (* eas ., *)
+                   admit. (* fun_map_inv *)
+                   (* fun_map_inv d (occurs_free_fundefs f2) (add_fundefs f2 fm) rho1' x2 j
+                      (set_list (combine (all_fun_name f2) xs) sig) *)
+             - inv HIn. contradiction. rewrite def_funs_neq in Hgetx; [| eassumption ]. eapply Henv in Hgetx; [| eassumption ]. destructAll. 
+               eexists. rewrite apply_r_set_list_f_eq. rewrite extend_lst_gso. rewrite def_funs_neq. 
+               split; eauto. eapply preord_val_monotonic. eassumption. omega. 
+               + intros Hc. eapply Same_set_all_fun_name in Hc. rewrite H12 in Hc.
+                 rewrite apply_r_list_eq in Hc; [| | now eauto ]. eapply Hdis2. constructor. 
+                 2:{ right. eapply In_image. now left; eauto. } 
+                 eapply fresh_Range. 2:{ eapply Hsub. eassumption. } eassumption. eassumption.
+               + rewrite <- Same_set_all_fun_name. intros Hc. eapply Hdis1. constructor. normalize_bound_var. left.
+                 now eapply name_in_fundefs_bound_var_fundefs. now eauto. }
+        -- repeat normalize_bound_var_in_ctx. repeat normalize_occurs_free_in_ctx.
+           rewrite Dom_map_def_funs. eapply Union_Disjoint_r.
+           ++ eapply Disjoint_Included_r. eapply name_in_fundefs_bound_var_fundefs. sets.
+           ++ sets.
+        -- admit. (* fun_map_inv *)
+           (* fun_map_inv d (occurs_free e) (add_fundefs f2 fm)
+                (def_funs f2 f2 rho1 rho1) (def_funs fds' fds' rho2 rho2) 
+                (k - 1) (set_list (combine (all_fun_name f2) xs) sig) *)
     - (* Eapp *)
       simpl. destruct (update_App St IH (apply_r sig v) t (apply_r_list sig l) st) as [s b] eqn:Hup. 
       + destruct b.
         * destruct (fm ! v) as [[[ft xs] e] |] eqn:Heqf.
           destruct d.
           -- eapply return_triple.
-             intros. split; [| split; [| split; [| split ]]]; try eassumption.
-             ++ constructor.
-             ++ simpl. repeat normalize_occurs_free. rewrite !image_Union, image_Singleton.
+             intros. split; [| split; [| split; [| split; [| split ]]]]; try eassumption.
+             ++ reflexivity.
+             ++ constructor. 
+             ++ repeat normalize_occurs_free. rewrite !image_Union, image_Singleton.
                 rewrite FromList_apply_list. sets.
              ++ normalize_bound_var. sets.
              ++ intros. eapply preord_exp_app_compat.
@@ -938,7 +1139,7 @@ Section Inline_correct.
              { symmetry in Hbeq. eapply beq_nat_eq in Hbeq.
                edestruct Hfm. eassumption. destructAll. eapply post_weakening; [| eapply IHd ].
                ++ simpl. intros. destructAll. 
-                  split; [| split; [| split; [| split ]]]; try eassumption.
+                  split; [| split; [| split; [| split; [| split ]]]]; try eassumption.
                   ** eapply Included_trans. eassumption. 
                      eapply Included_trans. eapply image_apply_r_set_list.
                      unfold apply_r_list. rewrite list_length_map. eassumption.
@@ -948,54 +1149,25 @@ Section Inline_correct.
                      eapply Union_Included; [| now sets ].
                      eapply image_monotonic. intros z Hin. do 4 eexists; split; eauto.
                   ** intros. eapply preord_exp_app_l.
-                   --- admit. (* post *)
-                   --- admit. (* post *)
-                   --- intros. assert (Hf := H12). assert (Heqf' := Heqf). edestruct H12; eauto. destructAll.
-                       do 2 subst_exp. eapply H8.
-                       +++ edestruct preord_env_P_inj_get_list_l. now eapply H9. normalize_occurs_free. now sets.
-                           eassumption. destructAll.                           
-                           eapply preord_env_P_inj_set_lists_l'; try eassumption. eapply preord_env_P_inj_antimon. eassumption.
-                           eapply Setminus_Included_Included_Union. eapply Included_trans. eapply occurs_free_in_fun.
-                           eapply find_def_correct. eassumption. sets.
-                       +++ erewrite Dom_map_set_lists; [| eassumption ]. rewrite Dom_map_def_funs.
-                           eapply Union_Disjoint_r; [| now xsets ].
-                           eapply Disjoint_Included_r. eapply occurs_free_in_env_set_lists_not_In. eassumption.
-                           eapply Disjoint_Included_r. eapply Included_Union_compat. reflexivity.
-                           eapply sub_map_occurs_free_in_env. eassumption.
-                           rewrite Union_Same_set. now sets. eapply occurs_free_in_env_get_list. eassumption.
-                       +++ eapply Disjoint_Included_r. eapply image_apply_r_set_list.
-                           unfold apply_r_list. rewrite list_length_map. eassumption.
-                           eapply Union_Disjoint_r.
-                           eapply Disjoint_Included_r; [|  eapply Hdis2 ]. normalize_occurs_free. rewrite image_Union.
-                           rewrite FromList_apply_list. now sets.
-                           eapply Disjoint_Included_r. eapply image_monotonic. eapply Setminus_Included.
-                           eapply Disjoint_Included_r. eapply image_monotonic.
-                           eapply occurs_free_in_env_set_lists_not_In. eassumption.
-                           rewrite image_Union. eapply Union_Disjoint_r.
-                           eapply Disjoint_Included_r; [|  eapply H11 ]. eapply image_monotonic.
-                           eapply occurs_free_in_env_get_list. eassumption.
-                           eapply Disjoint_Included_r; [| eapply H11 ]. eapply image_monotonic.
-                           eapply sub_map_occurs_free_in_env. eassumption. 
-                       +++ eapply fun_map_inv_antimon. eapply fun_map_inv_set_lists; [ | | | | | | | eassumption ].
-                           *** rewrite <- fun_map_inv_eq in *. eapply H23.
-                           *** eapply fun_map_inv_mon. eapply Hf. omega.
-                           *** sets.
-                           *** eapply occurs_free_in_env_get_list. eassumption.
-                           *** eassumption.
-                           *** eassumption. 
-                           *** rewrite Dom_map_def_funs. xsets.
-                           *** eapply Included_trans. eapply Included_Union_compat. reflexivity.
-                               eapply occurs_free_in_env_set_lists_not_In. eassumption.
-                               eapply Union_Included; [| eapply Union_Included ]. 
-                               ++++ eapply Included_trans.
-                                    2:{ eapply Included_Union_compat. reflexivity. eapply occurs_free_in_env_get. eapply H14. }
-                                    eapply Included_trans. eapply occurs_free_in_fun. eapply find_def_correct. eassumption.
-                                    sets.
-                               ++++ eapply Included_trans. eapply occurs_free_in_env_get_list. eassumption. sets.
-                               ++++ eapply Included_trans. eapply sub_map_occurs_free_in_env. eassumption. sets.
+                     --- admit. (* post *)
+                     --- admit. (* post *)
+                     --- intros. assert (Hf := H12). assert (Heqf' := Heqf). edestruct H12; eauto. destructAll.
+                         do 2 subst_exp. eapply H9.
+                         +++ edestruct preord_env_P_inj_get_list_l. now eapply H10. normalize_occurs_free. now sets.
+                             eassumption. destructAll.                           
+                             eapply preord_env_P_inj_set_lists_l'; try eassumption.
+                         +++ erewrite Dom_map_set_lists; [| eassumption ]. rewrite Dom_map_def_funs. xsets.
+                         +++ eapply fun_map_inv_antimon. eapply fun_map_inv_set_lists; [ | | | | | | eassumption ].
+                             *** rewrite <- fun_map_inv_eq in *. eapply H23.
+                             *** rewrite <- fun_map_inv_eq in *. eapply H23.
+                             *** sets.
+                             *** eapply sub_map_refl.
+                             *** eassumption. 
+                             *** rewrite Dom_map_def_funs. xsets.
+                             *** rewrite Union_Setminus_Included. sets. tci. sets.
                ++ omega.
                ++ eassumption.
-               ++ eassumption.
+               ++ sets.
                ++ eapply Union_Disjoint_r. now sets.
                   eapply Disjoint_Included_r. eapply image_apply_r_set_list.
                   unfold apply_r_list. rewrite list_length_map. eassumption.
@@ -1003,15 +1175,16 @@ Section Inline_correct.
                   eapply Disjoint_Included_r; [| eapply Hdis2 ]. normalize_occurs_free.
                   rewrite image_Union. rewrite FromList_apply_list. now sets. now sets.
                ++ (* Make lemma if needed about fun_map_vars fm S (set_list (combine xs (apply_r_list sig l)) sig) *)
-                  intros ? ? ? ? ?. edestruct Hfm; eauto. destructAll.
-                  repeat (split; [ now eauto |]). eapply Union_Disjoint_r. now sets.
-                  eapply Disjoint_Included_r. eapply image_apply_r_set_list.
-                  unfold apply_r_list. rewrite list_length_map. eassumption.
-                  eapply Union_Disjoint_r.
-                  eapply Disjoint_Included_r; [| eapply Hdis2 ]. normalize_occurs_free.
-                  rewrite image_Union. rewrite FromList_apply_list. now sets. now sets. }
-             { eapply return_triple.
-               intros. split; [| split; [| split; [| split ]]]; try eassumption.
+                 intros ? ? ? ? ?. edestruct Hfm; eauto. destructAll.
+                 repeat (split; [ now eauto |]). eapply Union_Disjoint_r. now sets.
+                 eapply Disjoint_Included_r. eapply image_apply_r_set_list.
+                 unfold apply_r_list. rewrite list_length_map. eassumption.
+                 eapply Union_Disjoint_r.
+                 eapply Disjoint_Included_r; [| eapply Hdis2 ]. normalize_occurs_free.
+                 rewrite image_Union. rewrite FromList_apply_list. now sets. now sets. }
+             { eapply return_triple. 
+               intros. split; [| split; [| split; [| split; [| split ]]]]; try eassumption.
+               ++ reflexivity.
                ++ constructor.
                ++ simpl. repeat normalize_occurs_free. rewrite !image_Union, image_Singleton.
                   rewrite FromList_apply_list. sets.
@@ -1022,7 +1195,8 @@ Section Inline_correct.
                   eapply Forall2_preord_var_env_map. eassumption.
                   now constructor. }
           -- eapply return_triple.
-             intros. split; [| split; [| split; [| split ]]]; try eassumption.
+             intros. split; [| split; [| split; [| split; [| split ]]]]; try eassumption.
+             ++ reflexivity.
              ++ constructor.
              ++ simpl. repeat normalize_occurs_free. rewrite !image_Union, image_Singleton.
                 rewrite FromList_apply_list. sets.
@@ -1033,7 +1207,8 @@ Section Inline_correct.
                 eapply Forall2_preord_var_env_map. eassumption.
                 now constructor.
         *  eapply return_triple.
-           intros. split; [| split; [| split; [| split ]]]; try eassumption.
+           intros. split; [| split; [| split; [| split; [| split ]]]]; try eassumption.
+           ++ reflexivity.
            ++ constructor.
            ++ simpl. repeat normalize_occurs_free. rewrite !image_Union, image_Singleton.
               rewrite FromList_apply_list. sets.
