theories/L6_PCPS/shrink_cps_corresp.v
@@ -4580,17 +4580,6 @@ Section CONTRACT.
     - sets.
   Qed.
 
-  Theorem apply_r_list_In:
-    forall v1 sig l,
-      List.In v1 l ->
-      List.In (apply_r sig v1) (apply_r_list sig l).
-  Proof.
-    induction l.
-    intro. inv H.
-    intros. inv H.
-    simpl. auto.
-    apply IHl in H0. simpl. auto.
-  Qed.
 
   Theorem inlined_fundefs_ctx_append1:
     forall v f l fds_c im fds,
